Towards type preservation for composed vlsms

composed_vlsm.v
@@ -5,18 +5,39 @@ From Casper
 Require Import vlsm two_vlsms list_of_vlsms indexed_vlsm.
 
 
+Definition noneOrAll
+  (op : option Prop)
+  : Prop
+  :=
+  match op with
+  | None => True
+  | (Some p) => p
+  end.
+
+
 Class composed_vlsm_class (message : Type) `{VLSM message} :=
   { index : Set
   ; iproto_state : index -> Type
   ; istate_proj : forall i : index, state -> iproto_state i
   ; ilabel : label -> index
-  ; valid_transition_projection_consistency
+  ; iproto_message_prop : index -> message -> Prop
+  ; iproto_message_decidable : forall i : index, forall m : message, {iproto_message_prop i m} + {~iproto_message_prop i m}
+  ; iproto_message_inhabited : forall i : index, inhabited {m : message | iproto_message_prop i m}
+  ; iproto_message_consistent : forall i : index, forall m : message, iproto_message_prop i m -> proto_message_prop m
+
+  ; transition_projection_consistency
     : forall (s1 s2 : state) (om : option proto_message) (l : label) (i : index)
         (Hproj_s : istate_proj i s1 = istate_proj i s2)
         (Hli : ilabel l = i),
     (   snd (transition l (s1, om)) = snd (transition l (s2, om))
     /\  istate_proj i (fst (transition l (s1, om))) = istate_proj i (fst (transition l (s2, om)))
     )
+(*
+  ; transition_projection_type_preservation
+    : forall (s : state) (om : option proto_message) (l : label) (i : index)
+        (Hli : ilabel l = i),
+        noneOrAll (option_map (iproto_message_prop i) (option_map (@proj1_sig message proto_message_prop) (snd (transition l (s, om)))))
+*)
   }.
 
 Definition istate
@@ -86,7 +107,49 @@ Definition composed2_ilabel
   | inr _ => two
   end.
 
-Lemma composed2_valid_transition_projection_consistency
+Definition composed2_iproto_message_prop
+  {message}
+  (S1 : VLSM message)
+  (S2 : VLSM message)
+  (i : composed2_index)
+  : message -> Prop
+  :=
+  match i with
+  | one => @proto_message_prop message S1
+  | two => @proto_message_prop message S2
+  end.
+
+Lemma composed2_iproto_message_decidable
+  {message}
+  (S1 : VLSM message)
+  (S2 : VLSM message)
+  (i : composed2_index)
+  : forall m : message, {composed2_iproto_message_prop S1 S2 i m} + {~composed2_iproto_message_prop S1 S2 i m}.
+Proof.
+  unfold composed2_iproto_message_prop. destruct i; apply proto_message_decidable.
+Qed.
+
+Lemma composed2_iproto_message_inhabited
+  {message}
+  (S1 : VLSM message)
+  (S2 : VLSM message)
+  (i : composed2_index)
+  : inhabited {m : message | composed2_iproto_message_prop S1 S2 i m}.
+Proof.
+  unfold composed2_iproto_message_prop. destruct i; apply message_inhabited.
+Qed.
+
+Lemma composed2_iproto_message_consistent
+  {message}
+  (S1 : VLSM message)
+  (S2 : VLSM message)
+  (i : composed2_index)
+  : forall m : message, composed2_iproto_message_prop S1 S2 i m -> composed2_proto_message_prop S1 S2 m.
+Proof.
+  unfold composed2_iproto_message_prop; intros. destruct i; (left; assumption) || (right; assumption).
+Qed.
+
+Lemma composed2_transition_projection_consistency
   {message}
   (S1 : VLSM message)
   (S2 : VLSM message)
@@ -108,6 +171,35 @@ Proof.
   destruct (proto_message_decidable m) as [Hpm | Hnpm]; simpl; split; reflexivity.
 Qed.
 
+Lemma composed2_transition_projection_type_preservation
+  {message}
+  (S1 : VLSM message)
+  (S2 : VLSM message)
+  : forall
+      (s : @state message S1 * @state message S2)
+      (om : option (composed2_proto_message S1 S2))
+      (l : @label message S1 + @label message S2)
+      (i : composed2_index)
+      (Hli : composed2_ilabel S1 S2 l = i),
+      noneOrAll
+        (option_map (composed2_iproto_message_prop S1 S2 i)
+          (option_map (@proj1_sig message (composed2_proto_message_prop S1 S2))
+            (snd (composed2_transition S1 S2 l (s, om)))))
+  .
+Proof.
+  intros.
+  destruct s as [sone stwo]. destruct l as [lone | ltwo]; simpl in Hli; subst; destruct om as [[m Hm]|]; simpl in *; subst
+  ; try (destruct (proto_message_decidable m) as [Hpm | Hnpm]; simpl); try exact I.
+  - remember (transition lone (sone, Some (exist proto_message_prop m Hpm))) as t.
+    destruct t as (s', om'). destruct om' as [[m' Hpm']|]; simpl; try assumption; try exact I.
+  - remember (transition lone (sone, None)) as t.
+    destruct t as (s', om'). destruct om' as [[m' Hpm']|]; simpl; try assumption; try exact I.
+  - remember (transition ltwo (stwo, Some (exist proto_message_prop m Hpm))) as t.
+    destruct t as (s', om'). destruct om' as [[m' Hpm']|]; simpl; try assumption; try exact I.
+  - remember (transition ltwo (stwo, None)) as t.
+    destruct t as (s', om'). destruct om' as [[m' Hpm']|]; simpl; try assumption; try exact I.
+Qed.
+
 Definition composed2_vlsm_composed_instance
   {message}
   (S1 : VLSM message)
@@ -117,9 +209,12 @@ Definition composed2_vlsm_composed_instance
   ; iproto_state := composed2_iproto_state S1 S2
   ; istate_proj := composed2_istate_proj' S1 S2
   ; ilabel := composed2_ilabel S1 S2
-  ; valid_transition_projection_consistency := composed2_valid_transition_projection_consistency S1 S2
+  ; iproto_message_prop := composed2_iproto_message_prop S1 S2
+  ; iproto_message_decidable := composed2_iproto_message_decidable S1 S2
+  ; iproto_message_inhabited := composed2_iproto_message_inhabited S1 S2
+  ; iproto_message_consistent := composed2_iproto_message_consistent S1 S2
+  ; transition_projection_consistency := composed2_transition_projection_consistency S1 S2
   |}.
-
 
 Definition composed2_constrained_istate_proj
   {message}
@@ -145,7 +240,11 @@ Definition composed2_vlsm_constrained_composed_instance
   ; iproto_state := composed2_iproto_state S1 S2
   ; istate_proj := composed2_constrained_istate_proj S1 S2 constraint constraint_decidable
   ; ilabel := composed2_ilabel S1 S2
-  ; valid_transition_projection_consistency := composed2_valid_transition_projection_consistency S1 S2
+  ; iproto_message_prop := composed2_iproto_message_prop S1 S2
+  ; iproto_message_decidable := composed2_iproto_message_decidable S1 S2
+  ; iproto_message_inhabited := composed2_iproto_message_inhabited S1 S2
+  ; iproto_message_consistent := composed2_iproto_message_consistent S1 S2
+  ; transition_projection_consistency := composed2_transition_projection_consistency S1 S2
   |}.
 
 Definition composed_list_index
@@ -209,7 +308,61 @@ destruct l as [lh | lt].
   exact (exist _ (S i) Hi).
 Defined.
 
-Lemma composed_list_valid_transition_projection_consistency
+Fixpoint composed_list_iproto_message_prop
+  {message}
+  (Ss : list (VLSM message))
+  : composed_list_index Ss -> message -> Prop.
+intros [i Hi] m.
+destruct Ss as [| Sh St].
+- exfalso. inversion Hi.
+- destruct i.
+  + exact (@proto_message_prop message Sh m).
+  + specialize (composed_list_iproto_message_prop message St).
+    specialize (composed_list_iproto_message_prop (exist _ i (le_pred _ _ Hi))).
+    exact (composed_list_iproto_message_prop m).
+Defined.
+
+Lemma composed_list_iproto_message_decidable
+  {message}
+  (Ss : list (VLSM message))
+  (i : composed_list_index Ss)
+  : forall m : message, {composed_list_iproto_message_prop Ss i m} + {~composed_list_iproto_message_prop Ss i m}.
+Proof.
+  induction Ss; destruct i as [i Hi].
+  - exfalso. inversion Hi.
+  - destruct i; simpl; try apply proto_message_decidable.
+    specialize (IHSs  (exist _ i (le_pred _ _ Hi))); simpl in IHSs.
+    assumption.
+Qed.
+
+Lemma composed_list_iproto_message_inhabited
+  {message}
+  (Ss : list (VLSM message))
+  (i : composed_list_index Ss)
+  : inhabited {m : message | composed_list_iproto_message_prop Ss i m}.
+Proof.
+  induction Ss; destruct i as [i Hi].
+  - exfalso. inversion Hi.
+  - destruct i; simpl; try apply message_inhabited.
+    specialize (IHSs  (exist _ i (le_pred _ _ Hi))); simpl in IHSs.
+    assumption.
+Qed.
+
+Lemma composed_list_iproto_message_consistent
+  {message}
+  (Ss : list (VLSM message))
+  (i : composed_list_index Ss)
+  : forall m : message, composed_list_iproto_message_prop Ss i m -> composed_list_proto_message_prop Ss m.
+Proof.
+  induction Ss; destruct i as [i Hi].
+  - exfalso. inversion Hi.
+  - destruct i; simpl; intros.
+    + left. assumption.
+    + right. specialize (IHSs (exist _ i (le_pred _ _ Hi)) m). simpl in IHSs.
+      apply IHSs. assumption.
+Qed.
+
+Lemma composed_list_transition_projection_consistency
   {message}
   (Ss : list (VLSM message))
   : forall
@@ -235,8 +388,21 @@ Proof.
   - simpl in Hproj_s. simpl in Hi.
     destruct l as [lh | lt].
     +  simpl in Hli. inversion Hli.
-    + destruct om as [[m Hm]|]. simpl.
-      * admit.
+    + destruct om as [[m Hm]|].
+      * simpl. destruct (composed_list_proto_message_decidable Ss m) as [Hpm | Hnpm]; simpl; try (split; reflexivity || assumption).
+        specialize (IHSs s1t s2t (Some (exist _ m Hpm)) lt (exist _ i (le_pred _ _ Hi)) Hproj_s).
+        simpl in Hli.
+        remember (composed_list_ilabel Ss lt) as j.
+        destruct j as [j Hj].
+        inversion Hli; subst.
+        assert
+          (Hirrelevant :
+            exist (fun n : nat => n < length Ss) i Hj =
+            exist (fun n : nat => n < length Ss) i (le_pred (S (S i)) (S (length Ss)) Hi)
+          ) by ( apply f_equal; apply proof_irrelevance ).
+        specialize (IHSs Hirrelevant).
+        destruct IHSs as [Hmsg' Hs'].
+        split; try assumption. simpl. apply f_equal. assumption.
       * specialize (IHSs s1t s2t None lt (exist _ i (le_pred _ _ Hi)) Hproj_s).
         simpl in Hli. 
         remember (composed_list_ilabel Ss lt) as j.
@@ -247,10 +413,10 @@ Proof.
             exist (fun n : nat => n < length Ss) i Hj =
             exist (fun n : nat => n < length Ss) i (le_pred (S (S i)) (S (length Ss)) Hi)
           ) by ( apply f_equal; apply proof_irrelevance ).
-      specialize (IHSs Hirrelevant).
-      destruct IHSs as [Hmsg' Hs'].
-      split; try assumption. simpl. apply f_equal. assumption.
-Admitted.
+        specialize (IHSs Hirrelevant).
+        destruct IHSs as [Hmsg' Hs'].
+        split; try assumption. simpl. apply f_equal. assumption.
+Qed.
 
 Definition composed_list_vlsm_composed_instance
   {message}
@@ -261,7 +427,11 @@ Definition composed_list_vlsm_composed_instance
   ; iproto_state := composed_list_iproto_state Ss
   ; istate_proj := composed_list_istate_proj' Ss Ssnn
   ; ilabel := composed_list_ilabel Ss
-  ; valid_transition_projection_consistency := composed_list_valid_transition_projection_consistency Ss
+  ; iproto_message_prop := composed_list_iproto_message_prop Ss
+  ; iproto_message_decidable := composed_list_iproto_message_decidable Ss
+  ; iproto_message_inhabited := composed_list_iproto_message_inhabited Ss
+  ; iproto_message_consistent := composed_list_iproto_message_consistent Ss
+  ; transition_projection_consistency := composed_list_transition_projection_consistency Ss
   |}.
 
 Definition composed_list_constrained_istate_proj
@@ -287,7 +457,11 @@ Definition composed_list_vlsm_constrained_composed_instance
   ; iproto_state := composed_list_iproto_state Ss
   ; istate_proj := composed_list_constrained_istate_proj Ss Ssnn constraint constraint_decidable
   ; ilabel := composed_list_ilabel Ss
-  ; valid_transition_projection_consistency := composed_list_valid_transition_projection_consistency Ss
+  ; iproto_message_prop := composed_list_iproto_message_prop Ss
+  ; iproto_message_decidable := composed_list_iproto_message_decidable Ss
+  ; iproto_message_inhabited := composed_list_iproto_message_inhabited Ss
+  ; iproto_message_consistent := composed_list_iproto_message_consistent Ss
+  ; transition_projection_consistency := composed_list_transition_projection_consistency Ss
   |}.
 
 Definition indexed_vlsm_istate
@@ -326,7 +500,44 @@ Definition indexed_vlsm_ilabel
   :=
   projT1 l.
 
-Lemma indexed_vlsm_valid_transition_projection_consistency
+Definition indexed_vlsm_iproto_message_prop
+  {oindex : Set} {message : Type} `{Heqd : EqDec oindex}
+  {IS : oindex -> VLSM message}
+  (i : oindex)
+  : message -> Prop
+  :=
+  @proto_message_prop message (IS i).
+
+Definition indexed_vlsm_iproto_message_decidable
+  {oindex : Set} {message : Type} `{Heqd : EqDec oindex}
+  {IS : oindex -> VLSM message}
+  (i : oindex)
+  : forall m : message, {indexed_vlsm_iproto_message_prop i m} + {~indexed_vlsm_iproto_message_prop i m}
+  :=
+  @proto_message_decidable message (IS i).
+
+Definition indexed_vlsm_iproto_message_inhabited
+  {oindex : Set} {message : Type} `{Heqd : EqDec oindex}
+  {IS : oindex -> VLSM message}
+  (i : oindex)
+  : inhabited {m : message | indexed_vlsm_iproto_message_prop i m}
+  :=
+  @message_inhabited message (IS i).
+
+Lemma indexed_vlsm_iproto_message_consistent
+  {index : Set} {message : Type} `{Heqd : EqDec index}
+  {IS : index -> VLSM message}
+  (i : index)
+  : forall m : message,
+  indexed_vlsm_iproto_message_prop i m ->
+  @proto_message_prop message (indexed_vlsm IS (inhabits i)) m.
+Proof.
+  unfold indexed_vlsm_iproto_message_prop.
+  intros m Hmi.
+  exists i. assumption.
+Qed.
+
+Lemma indexed_vlsm_transition_projection_consistency
   {oindex : Set} {message : Type} `{Heqd : EqDec oindex}
   {IS : oindex -> VLSM message}
   : forall
@@ -340,7 +551,25 @@ Lemma indexed_vlsm_valid_transition_projection_consistency
     /\  indexed_vlsm_istate_proj i (fst (indexed_transition IS l (s1, om)))
       = indexed_vlsm_istate_proj i (fst (indexed_transition IS l (s2, om)))
     ).
-Admitted.
+Proof.
+  intros.
+  destruct l as [j l]. simpl in Hli. subst.
+  unfold indexed_vlsm_istate_proj in Hproj_s.
+  unfold indexed_vlsm_istate_proj.
+  simpl.
+  destruct om as [[m Hm]|].
+  - destruct (proto_message_decidable m) as [Hpm | Hnpm]; simpl; try (split; reflexivity || assumption).
+    rewrite <- Hproj_s. 
+    remember (transition l (s1 i, Some (exist proto_message_prop m Hpm))) as t.
+    destruct t as [si' om']. simpl. split; try reflexivity.
+    destruct (eq_dec i i); try contradiction.
+    reflexivity.
+  - rewrite <- Hproj_s.
+    remember (transition l (s1 i, None)) as t.
+    destruct t as [si' om']. simpl. split; try reflexivity.
+    destruct (eq_dec i i); try contradiction.
+    reflexivity.
+Qed.
 
 Definition indexed_vlsm_composed_instance
   {oindex : Set} {message : Type} `{Heqd : EqDec oindex}
@@ -351,7 +580,11 @@ Definition indexed_vlsm_composed_instance
   ; iproto_state := @indexed_vlsm_istate oindex message Heqd IS
   ; istate_proj := @indexed_vlsm_istate_proj' oindex message Heqd IS Hi
   ; ilabel := indexed_vlsm_ilabel
-  ; valid_transition_projection_consistency := indexed_vlsm_valid_transition_projection_consistency
+  ; iproto_message_prop := indexed_vlsm_iproto_message_prop
+  ; iproto_message_decidable := indexed_vlsm_iproto_message_decidable
+  ; iproto_message_inhabited := indexed_vlsm_iproto_message_inhabited
+  ; iproto_message_consistent := indexed_vlsm_iproto_message_consistent
+  ; transition_projection_consistency := indexed_vlsm_transition_projection_consistency
   |}.
 
 Definition indexed_vlsm_constrained_istate_proj
@@ -377,5 +610,9 @@ Definition indexed_vlsm_constrained_composed_instance
   ; iproto_state := @indexed_vlsm_istate oindex message Heqd IS
   ; istate_proj := @indexed_vlsm_constrained_istate_proj oindex message Heqd IS Hi constraint constraint_decidable
   ; ilabel := indexed_vlsm_ilabel
-  ; valid_transition_projection_consistency := indexed_vlsm_valid_transition_projection_consistency
+  ; iproto_message_prop := indexed_vlsm_iproto_message_prop
+  ; iproto_message_decidable := indexed_vlsm_iproto_message_decidable
+  ; iproto_message_inhabited := indexed_vlsm_iproto_message_inhabited
+  ; iproto_message_consistent := indexed_vlsm_iproto_message_consistent
+  ; transition_projection_consistency := indexed_vlsm_transition_projection_consistency
   |}.
